Progress

x86/Asm.v
@@ -235,7 +235,7 @@ Inductive instruction: Type :=
   (** Branches and calls *)
   | Pjmp_l (l: label)
   | Pjmp_s (symb: ident) (sg: signature)
-  | Pjmp_r (r: ireg) (sg: signature) (checkfunzero: bool)
+  | Pjmp_r (r: ireg) (sg: signature)
   | Pjcc (c: testcond)(l: label)
   | Pjcc2 (c1 c2: testcond)(l: label)   (**r pseudo *)
   | Pjmptbl (r: ireg) (tbl: list label) (**r pseudo *)
@@ -1052,13 +1052,11 @@ Definition exec_instr {exec_load exec_store} `{!MemAccessors exec_load exec_stor
       goto_label ge f lbl rs m
   | Pjmp_s id sg =>
       Next (rs#PC <- (Genv.symbol_address ge id Ptrofs.zero)) m
-  | Pjmp_r r sg checkfunzero =>
-    if checkfunzero
-    then match Genv.find_funct ge (rs r) with
-         | Some _ => Next (rs#PC <- (rs r)) m
-         | _ => Stuck
-         end
-    else Next (rs#PC <- (rs r)) m
+  | Pjmp_r r sg =>
+    match Genv.find_funct ge (rs r) with
+    | Some _ => Next (rs#PC <- (rs r)) m
+    | _ => Stuck
+    end
   | Pjcc cond lbl =>
       match eval_testcond cond rs with
       | Some true => goto_label ge f lbl rs m
@@ -1247,6 +1245,13 @@ Definition loc_external_result (sg: signature) : rpair preg :=
 
 Inductive state {memory_model_ops: Mem.MemoryModelOps mem}: Type :=
   | State: regset -> mem -> state.
+
+Fixpoint in_builtin_res (b: builtin_res preg) (r:preg) :=
+  match b with
+  | BR b => b = r
+  | BR_none => False
+  | BR_splitlong hi lo => in_builtin_res hi r \/ in_builtin_res lo r
+  end.
 
 Inductive step {exec_load exec_store} `{!MemAccessors exec_load exec_store} (ge: genv)
             : state -> trace -> state -> Prop :=
@@ -1530,7 +1535,7 @@ Definition instr_to_string (i:instruction) : string :=
   (* (** Branches and calls *) *)
   | Pjmp_l l  => "Pjmp_l"
   | Pjmp_s symb sg => "Pjmp_s"
-  | Pjmp_r r sg checkfunzero  => "Pjmp_r"
+  | Pjmp_r r sg  => "Pjmp_r"
   | Pjcc c l => "Pjcc"
   | Pjcc2 c1 c2 l => "Pjcc2"  (**r pseudo *)
   | Pjmptbl r tbl => "Pjmptbl"  (**r pseudo *)
