x86/RawAsmMergeSteps.v
@@ -48,15 +48,14 @@ Section WITHGE.
   Definition m_state s :=
     let '(State _ m) := s in m.
 
-  Inductive is_call (rs: regset): instruction -> Prop :=
+  Inductive is_call: instruction -> Prop :=
   | is_call_s:
       forall symb b sg,
         Genv.find_symbol ge symb = Some b ->
-        is_call rs (Pcall_s symb sg)
+        is_call (Pcall_s symb sg)
   | is_call_r:
-      forall (r: ireg) b sg,
-        rs r = Vptr b Ptrofs.zero ->
-        is_call rs (Pcall_r r sg).
+      forall (r: ireg) sg,
+        is_call (Pcall_r r sg).
 
   Inductive is_alloc sz : instruction -> Prop :=
     is_alloc_intro f:
@@ -84,14 +83,18 @@ Section WITHGE.
         is_jmp (Pjmp_s symb sg)
   | is_jmp_r:
       forall (r: ireg) sg,
-        is_jmp (Pjmp_r r sg true).
+        is_jmp (Pjmp_r r sg).
+
+  Inductive intermediate_instruction : instruction -> Prop :=
+  | ii_alloc i sz: is_alloc sz i -> intermediate_instruction i
+  | ii_jmp i: i = Pret \/ is_jmp i -> intermediate_instruction i.
 
   Inductive step: state -> trace -> state -> Prop :=
   | step_call_internal:
       forall s1 s2 s3 f0 icall f ialloc
         (PC1: pc_at s1 = Some (inl (f0, icall)))
         (PC2: pc_at s2 = Some (inl (f, ialloc)))
-        (CALL: is_call (rs_state s1) icall)
+        (CALL: is_call icall)
         (ALLOC: is_alloc (frame_size (fn_frame f)) ialloc)
         (STEP1: RawAsm.step ge s1 E0 s2)
         (STEP2: RawAsm.step ge s2 E0 s3),
@@ -99,7 +102,7 @@ Section WITHGE.
   | step_call_external:
       forall s1 s2 s3 f0 icall ef t
         (PC1: pc_at s1 = Some (inl (f0, icall)))
-        (CALL: is_call (rs_state s1) icall)
+        (CALL: is_call icall)
         (PC2: pc_at s2 = Some (inr ef))
         (STEP1: RawAsm.step ge s1 E0 s2)
         (STEP2: RawAsm.step ge s2 t s3),
@@ -139,8 +142,8 @@ Section WITHGE.
       forall s1 t s2 r
         (PC: pc_at s1 = Some r)
         (NOFREE: forall f0 i, r = inl (f0,i) -> forall f, ~ is_free f i)
-        (NOFREE: forall f0 i, r = inl (f0,i) -> forall f, ~ is_alloc f i)
-        (NOCALL: forall f0 i, r = inl (f0,i) -> i <> Pret /\ ~ is_jmp i /\ ~ is_call (rs_state s1) i)
+        (NOFREE: forall f0 i, r = inl (f0,i) -> ~ intermediate_instruction i)
+        (NOCALL: forall f0 i, r = inl (f0,i) -> ~ is_call i)
         (STEP: RawAsm.step ge s1 t s2),
         step s1 t s2
   .
@@ -181,17 +184,14 @@ Section SIMU.
   Qed.
 
   Lemma is_call_dec:
-    forall rs i,
-      is_call ge rs i \/ ~ is_call ge rs i.
+    forall i,
+      is_call ge i \/ ~ is_call ge i.
   Proof.
     destruct i; try now (right; intro A; inv A).
     - destruct (Genv.find_symbol ge symb) eqn:FS.
       left; econstructor; eauto.
       right; intro A; inv A. congruence.
-    - destruct (rs r) eqn:PTR; try now (right; intro A; inv A; congruence).
-      destruct (Ptrofs.eq_dec i Ptrofs.zero). subst.
-      left; econstructor; eauto.
-      right; intro A; inv A; congruence.
+    - left; econstructor; eauto.
   Qed.
 
   Lemma is_free_dec:
@@ -206,6 +206,11 @@ Section SIMU.
 
   Inductive is_builtin: instruction -> Prop :=
   | is_builtin_intro ef args res: is_builtin (Pbuiltin ef args res).
+
+  Lemma is_builtin_dec i: is_builtin i \/ ~ is_builtin i.
+  Proof.
+    destruct i; first [right; now inversion 1|now econstructor].
+  Qed.
   
   Lemma step_internal:
     forall s t s'
@@ -243,6 +248,19 @@ Section SIMU.
                  | rewrite Asmgenproof0.nextinstr_inv by congruence
                  ].
 
+
+
+  Lemma set_res_other:
+    forall res vres rs r,
+      ~ in_builtin_res res r ->
+      set_res res vres rs r = rs r.
+  Proof.
+    induction res; simpl; intros; eauto.
+    rewrite Pregmap.gso; auto.
+    rewrite IHres2. apply IHres1. intuition. intuition.
+  Qed.
+
+  
   Record wf_asm_function (f: function): Prop :=
     {
       wf_asm_call_target_exists:
@@ -282,8 +300,21 @@ Section SIMU.
           exists o' ifree,
             find_instr (Ptrofs.unsigned o') (fn_code f) = Some ifree /\
             is_free (frame_size (fn_frame f)) ifree /\
-            Ptrofs.unsigned (Ptrofs.repr (instr_size (make_palloc (fn_frame f)))) <= Ptrofs.unsigned o' < Ptrofs.unsigned o;
-      
+            Ptrofs.unsigned o' + instr_size ifree = Ptrofs.unsigned o;
+
+      wf_asm_pc_repr:
+        forall i o,
+          find_instr (Ptrofs.unsigned o) (fn_code f) = Some i ->
+          Ptrofs.unsigned (Ptrofs.add o (Ptrofs.repr (instr_size i))) = Ptrofs.unsigned o + instr_size i;
+
+      wf_asm_code_bounded:
+        0 <= code_size (fn_code f) <= Ptrofs.max_unsigned;
+
+      wf_asm_builtin_not_PC:
+        forall o ef args res,
+          find_instr o (fn_code f) = Some (Pbuiltin ef args res) ->
+          ~ in_builtin_res res PC;
+
     }.
 
   Hypothesis wf_asm_prog:
@@ -308,10 +339,6 @@ Section SIMU.
     unfold Vnullptr in PCAT. destruct (ptr64); inv PCAT.
   Qed.
 
-  Inductive intermediate_instruction : instruction -> Prop :=
-  | ii_ret: intermediate_instruction Pret
-  | ii_alloc i sz: is_alloc sz i -> intermediate_instruction i
-  | ii_jmp i: is_jmp ge i -> intermediate_instruction i.
 
 
   Axiom instr_size_repr:
@@ -340,19 +367,227 @@ Section SIMU.
     - apply find_instr_pos_positive in H3. omega.
     - specialize (IHl _ _ _ _ H3 H2). trim IHl. omega. omega.
   Qed.
+
+  Lemma find_instr_no_overlap':
+    forall l o1 o2 i1 i2,
+      find_instr o1 l = Some i1 ->
+      find_instr o2 l = Some i2 ->
+      i1 = i2 \/ o1 + instr_size i1 <= o2 \/ o2 + instr_size i2 <= o1.
+  Proof.
+    intros l o1 o2 i1 i2 FI1 FI2.
+    destruct (zeq o1 o2). subst. rewrite FI1 in FI2; inv FI2; auto.
+    right.
+    eapply find_instr_no_overlap; eauto.
+  Qed.
+
+  Lemma intermediate_before:
+    forall f i0 i i1,
+      wf_asm_function f ->
+      find_instr (Ptrofs.unsigned (Ptrofs.add i0 (Ptrofs.repr (instr_size i)))) (fn_code f) = Some i1 ->
+      find_instr (Ptrofs.unsigned i0) (fn_code f) = Some i ->
+      intermediate_instruction ge i1 ->
+      intermediate_instruction ge i \/ is_call ge i \/ exists sz, is_free sz i.
+  Proof.
+    intros f i0 i i1 WF FI1 FI II1.
+    inv II1.
+    {
+      inv H. exploit wf_asm_alloc_only_at_beginning. eauto. apply FI1.
+      erewrite wf_asm_pc_repr; eauto.
+      generalize (Ptrofs.unsigned_range i0) (instr_size_positive i); omega.
+    }
+    {
+      exploit wf_asm_ret_jmp_comes_after_freeframe. eauto. 2: eauto. eauto.
+      intros (o' & ifree & FI' & IFREE & RNG).
+      generalize (find_instr_no_overlap' _ _ _ _ _ FI FI').
+      intros [EQ|RNG']. right; right; subst. eauto.
+      erewrite wf_asm_pc_repr in RNG; eauto.
+      generalize (instr_size_positive ifree) (instr_size_positive i); omega.
+    }
+  Qed.
+
+  Lemma exec_load_nextinstr:
+    forall chunk m a r rd sz r0 m0,
+      rd <> PC ->
+      exec_load ge chunk m a r rd sz = Next r0 m0 ->
+      r0 PC = Val.offset_ptr (r PC) sz.
+  Proof.
+    unfold exec_load; intros chunk m a r rd sz r0 m0 NOPC EL; repeat destr_in EL. simpl_regs.
+    auto.
+  Qed.
+
+  Lemma exec_store_nextinstr:
+    forall chunk m a r rd lrd sz r0 m0,
+      rd <> PC -> Forall (fun x => x <> PC) lrd ->
+      exec_store ge chunk m a r rd lrd sz = Next r0 m0 ->
+      r0 PC = Val.offset_ptr (r PC) sz.
+  Proof.
+    unfold exec_store; intros chunk m a r rd lrd sz r0 m0 NOPC NOTPC EL; repeat destr_in EL. simpl_regs.
+    rewrite Asmgenproof0.undef_regs_other. auto.
+    intros r' IN EQ; subst. rewrite Forall_forall in NOTPC; apply NOTPC in IN. congruence.
+  Qed.
+
+  Lemma label_pos_rng:
+    forall lbl c pos z,
+      label_pos lbl pos c = Some z ->
+      0 <= pos ->
+      0 <= z - pos <= code_size c.
+  Proof.
+    induction c; simpl; intros; eauto. congruence. repeat destr_in H.
+    generalize (code_size_non_neg c) (instr_size_positive a); omega.
+    apply IHc in H2.
+    generalize (instr_size_positive a); omega.
+    generalize (instr_size_positive a); omega.
+  Qed.
+
+  Lemma label_pos_repr:
+    forall lbl c pos z,
+      code_size c + pos <= Ptrofs.max_unsigned ->
+      0 <= pos ->
+      label_pos lbl pos c = Some z ->
+      Ptrofs.unsigned (Ptrofs.repr (z - pos)) = z - pos.
+  Proof.
+    intros.
+    apply Ptrofs.unsigned_repr.
+    generalize (label_pos_rng _ _ _ _ H1 H0). omega.
+  Qed.
+
+  Lemma find_instr_ofs_pos:
+    forall c o i,
+      find_instr o c = Some i ->
+      0 <= o.
+  Proof.
+    induction c; simpl; intros; repeat destr_in H.
+    omega. apply IHc in H1. generalize (instr_size_positive a); omega.
+  Qed. 
   
+  Lemma label_pos_spec:
+    forall lbl c pos z,
+      code_size c + pos <= Ptrofs.max_unsigned ->
+      0 <= pos ->
+      label_pos lbl pos c = Some z ->
+      find_instr ((z - pos) - instr_size (Plabel lbl)) c = Some (Plabel lbl).
+  Proof.
+    induction c; simpl; intros; repeat destr_in H1. 
+    destruct a; simpl in Heqb; try congruence. repeat destr_in Heqb.
+    apply pred_dec_true. omega.
+    eapply IHc in H3. 2: omega. 2: generalize (instr_size_positive a); omega.
+    generalize (find_instr_ofs_pos _ _ _ H3). intro.
+    rewrite pred_dec_false. 2: generalize (instr_size_positive a); omega.
+    rewrite <- H3. f_equal. omega.                  
+  Qed.
+
+  Lemma goto_label_PC:
+    forall f l r m r0 m0
+      (GL: goto_label ge f l r m = Next r0 m0)
+      b i
+      (PCbef: r PC = Vptr b i)
+      (FFP: Genv.find_funct_ptr ge b = Some (Internal f)) ,
+      (forall f0 i2,
+          pc_at ge (State r0 m0) = Some (inl (f0,i2)) ->
+          ~ intermediate_instruction ge i2)
+      /\ (forall ef,
+            pc_at ge (State r0 m0) = Some (inr ef) ->
+            False ).
+  Proof.
+    intros.
+    simpl.
+    unfold goto_label in GL.
+    rewrite PCbef, FFP in GL. destr_in GL. inv GL. simpl_regs. rewrite FFP.
+    destr. split. 2: inversion 1. intros f0 i2 EQ; inv EQ.
+    assert (EQz: Ptrofs.unsigned (Ptrofs.repr z) = z).
+    {
+      replace z with (z-0) by omega.
+      eapply label_pos_repr. rewrite Z.add_0_r. eapply wf_asm_code_bounded. eauto. omega. eauto.
+    } rewrite EQz in *.
+    generalize (label_pos_spec l (fn_code f0) 0 z). intro LPS; trim LPS.
+    rewrite Z.add_0_r. apply wf_asm_code_bounded; eauto. trim LPS. omega. trim LPS; auto.
+    generalize (find_instr_ofs_pos _ _ _ LPS).
+    intros POS II; inv II.
+    {
+      inv H. exploit wf_asm_alloc_only_at_beginning. eauto. apply Heqo0.
+      generalize (instr_size_positive (Plabel l)); omega.
+    }
+    {
+      exploit wf_asm_ret_jmp_comes_after_freeframe. eauto. 2: apply H.
+      rewrite EQz. eauto.
+      intros (o' & ifree & FI & IFREE & RNG).
+      generalize (find_instr_no_overlap' _ _ _ _ _ FI LPS).
+      intros [EQ|NOOV]. subst; inv IFREE.
+      rewrite EQz in *.
+      generalize (instr_size_positive ifree) (instr_size_positive (Plabel l)). omega.
+    }
+  Qed.
+
+  Lemma normal_steps_preserves_normal:
+    forall s1 f i s2,
+      pc_at ge s1 = Some (inl (f, i)) ->
+      ~ intermediate_instruction ge i ->
+      ~ is_call ge i ->
+      ~ (exists sz, is_free sz i) ->
+      exec_instr ge f i (rs_state s1) (m_state s1) = Next (rs_state s2) (m_state s2) ->
+      (forall f0 i0, pc_at ge s2 = Some (inl (f0, i0)) -> ~ intermediate_instruction ge i0) /\
+      (forall ef, pc_at ge s2 = Some (inr ef) -> False).
+  Proof.
+    intros s1 f i s2 PC1 INV NOTCALL NOTFREE EI.
+    unfold pc_at in *. repeat destr_in PC1. destr. simpl in *. subst.
+    destruct (Val.eq (r0 PC) (Val.offset_ptr (r PC) (Ptrofs.repr (instr_size i)))).
+    ++ rewrite e, Heqv; simpl. rewrite Heqo.
+       destr.
+       split. 2: inversion 1. intros f0 i2 FI; inv FI.
+       intro II; eapply intermediate_before in II; eauto.
+       destruct II as [II|[CALL|FRE]]; eauto.
+    ++ destruct i;
+         first
+           [ exfalso; simpl in EI; repeat destr_in EI; simpl_regs_in n; rewrite Heqv in n; simpl in n; congruence
+           | exfalso; simpl in EI; apply n; eapply exec_load_nextinstr; eauto; congruence
+           | exfalso; simpl in EI; apply n; eapply exec_store_nextinstr; eauto; congruence
+           |   exfalso; simpl in EI; apply n; eapply (fun pf pf' => exec_store_nextinstr _ _ _ _ _ _ _ _ _ pf pf' EI); eauto; repeat constructor; congruence
+           | idtac
+           ].
+       simpl in EI. unfold compare_ints in EI. inv EI. simpl_regs_in n. congruence.
+       simpl in EI. unfold compare_longs in EI. inv EI. simpl_regs_in n. congruence.
+       simpl in EI. unfold compare_ints in EI. inv EI. simpl_regs_in n. congruence.
+       simpl in EI. unfold compare_longs in EI. inv EI. simpl_regs_in n. congruence.
+       simpl in EI. unfold compare_ints in EI. inv EI. simpl_regs_in n. congruence.
+       simpl in EI. unfold compare_longs in EI. inv EI. simpl_regs_in n. congruence.
+       simpl in EI. unfold compare_ints in EI. inv EI. simpl_regs_in n. congruence.
+       simpl in EI. unfold compare_longs in EI. inv EI. simpl_regs_in n. congruence.
+       simpl in EI. exfalso. unfold compare_floats in EI. inv EI. apply n. simpl_regs.
+       repeat destr; simpl_regs; congruence.
+       simpl in EI. exfalso. unfold compare_floats32 in EI. inv EI. apply n. simpl_regs.
+       repeat destr; simpl_regs; congruence.
+       simpl in EI.
+       eapply goto_label_PC; eauto.
+       edestruct wf_asm_jmp_target_exists as (bf & f'  & SA & _); eauto. unfold Genv.symbol_address in SA; destr_in SA.
+       exfalso; apply INV; constructor. right; econstructor; eauto.
+       exfalso; apply INV; constructor. right; econstructor; eauto.
+       simpl in EI. repeat destr_in EI. eapply goto_label_PC; eauto. simpl_regs_in n. congruence.
+       simpl in EI. repeat destr_in EI. eapply goto_label_PC; eauto. simpl_regs_in n. congruence.
+       simpl_regs_in n; congruence.
+       simpl in EI. repeat destr_in EI. eapply goto_label_PC; eauto.
+       exfalso; apply NOTCALL.
+       edestruct wf_asm_call_target_exists as (bf & f'  & SA & _); eauto. unfold Genv.symbol_address in SA; destr_in SA.
+       econstructor; eauto.
+       exfalso; apply NOTCALL. econstructor.
+       exfalso; apply INV. constructor. auto.
+       simpl in *. inv EI. rewrite Heqv, Heqo, Heqo0.
+       split. 2: inversion 1. intros f0 i A; inv A; eauto.
+  Qed.
+
   Lemma group_progress:
     forall rs s1
       (SAFE : safe (RawAsm.semantics prog rs) s1)
-      (INV: forall f i, pc_at ge s1 = Some (inl (f, i)) -> ~ intermediate_instruction i),
+      (INV: forall f i, pc_at ge s1 = Some (inl (f, i)) -> ~ intermediate_instruction ge i)
+      (INV2: forall ef, pc_at ge s1 = Some (inr ef) -> False),
       (exists r, final_state s1 r) \/ (exists t s2, step (Genv.globalenv prog) s1 t s2 /\
-                                         forall f i, pc_at ge s2 = Some (inl (f, i)) -> ~ intermediate_instruction i).
+                                         (forall f i, pc_at ge s2 = Some (inl (f, i)) -> ~ intermediate_instruction ge i) /\
+                                         (forall ef, pc_at ge s2 = Some (inr ef) -> False)).
   Proof.
     intros.
     destruct (SAFE _  (star_refl _ _ _)) as [(r & FS)|(t & s2 & STEP)].
     eauto.
     destruct (pc_at ge s1) as [[[f i]|ef]|] eqn:PCs.
-    - destruct (is_call_dec (rs_state s1) i) as [CALL|NOTCALL].
+    - destruct (is_call_dec i) as [CALL|NOTCALL].
       + (* it's a call instruction : the next step is going to be either an external function or a Pallocframe. *)
         simpl in STEP.
         exploit step_internal; eauto. intro IB; inv IB; inv CALL. intros (EI & T0). subst.
@@ -360,7 +595,7 @@ Section SIMU.
         * inv FS. simpl in EI.
           inv CALL; simpl in EI; repeat destr_in EI.
           -- simpl_regs_in H. unfold Genv.symbol_address in H. repeat destr_in H.
-          -- simpl_regs_in H. rewrite H in H1. inv H1.
+          -- simpl_regs_in H. rewrite H in Heqo.  inv Heqo.
         * simpl in STEP2.
           assert (exists b f', Genv.find_funct_ptr ge b = Some f' /\
                           rs_state s2 PC = Vptr b Ptrofs.zero).
@@ -370,7 +605,7 @@ Section SIMU.
               eapply wf_asm_call_target_exists in Heqo0; eauto.
               destruct Heqo0 as (bf & f' & SA & FFP).
               inv STEP2; simpl in *; subst; simpl_regs; simpl_regs_in H0; eauto.
-            - simpl_regs. rewrite H in *. simpl in Heqo. destr_in Heqo. eauto.
+            - simpl_regs. unfold Genv.find_funct in Heqo; repeat destr_in Heqo. eauto.
           }
           destruct H as (b & f' & FFP & PC2).
           inversion STEP2; subst.
@@ -383,16 +618,25 @@ Section SIMU.
              erewrite wf_asm_alloc_at_beginning in H1; eauto. inv H1.
              simpl in H2. repeat destr_in H2. unfold ge in FFP; rewrite FFP in H0. inv H0.
              simpl_regs. rewrite PC2. simpl. unfold ge. rewrite FFP.
-             destr. inversion 1; subst. intro A.
+             destr. split; inversion 1; subst. intro A.
              rewrite Ptrofs.add_zero_l in Heqo0.
              inv A.
-             eapply wf_asm_ret_jmp_comes_after_freeframe in Heqo0; eauto.
-             destruct Heqo0 as (o' & ifree & FI & IFREE & RNG). omega.
-             inv H0. eapply wf_asm_alloc_only_at_beginning in Heqo0; eauto.
-             rewrite Ptrofs.unsigned_repr in Heqo0. generalize (instr_size_positive (make_palloc (fn_frame f1))). omega.
-             apply instr_size_repr.
-             eapply wf_asm_ret_jmp_comes_after_freeframe in Heqo0; eauto.
-             destruct Heqo0 as (o' & ifree & FI & IFREE & RNG). omega.
+             {
+               inv H0. exploit wf_asm_alloc_only_at_beginning. eauto. apply Heqo0.
+               rewrite Ptrofs.unsigned_repr by apply instr_size_repr.
+               unfold make_palloc. apply not_eq_sym. apply Z.lt_neq. apply instr_size_positive. 
+             }
+             {
+               exploit wf_asm_ret_jmp_comes_after_freeframe; eauto.
+               intros (o' & ifree & FI & IFREE & RNG).
+               exploit wf_asm_alloc_at_beginning; eauto.
+               intro FALLOC.
+               generalize (find_instr_no_overlap' _ _ _ _ _ FI FALLOC).
+               rewrite Ptrofs.unsigned_repr in RNG by apply instr_size_repr.
+               rewrite RNG.
+               intros [EQ|NOOV]. subst; inv IFREE.
+               generalize (instr_size_positive (make_palloc (fn_frame f1))) (instr_size_positive ifree). omega.
+             }
           -- simpl in *. rewrite_hyps.
              erewrite wf_asm_alloc_at_beginning in H1; eauto. inv H1. 
           -- simpl in PC2. rewrite_hyps.
@@ -406,16 +650,21 @@ Section SIMU.
              {
                inv CALL; simpl in EI; repeat destr_in EI; simpl_regs; rewrite Heqv; simpl; auto.
              }
-             rewrite H. rewrite Heqo. destr. inversion 1; subst.
+             rewrite H. rewrite Heqo. destr. split; inversion 1; subst.
              intro II; inv II.
-             eapply wf_asm_ret_jmp_comes_after_freeframe in Heqo1; eauto.
-             destruct Heqo1 as (o' & ifree & FO & IFREE & _ & RNG).
-             generalize (find_instr_no_overlap _ _ _ _ _ FO Heqo0). intro NOOV.
-             trim NOOV.
-             intro EQ; rewrite EQ in FO. rewrite Heqo0 in FO. inv FO. inv IFREE; inv CALL.
-             rewrite Ptrofs.add_unsigned in RNG. rewrite Ptrofs.unsigned_repr in RNG.
-             rewrite Ptrofs.unsigned_repr in RNG. 
-
+             {
+               inv H4. exploit wf_asm_alloc_only_at_beginning. eauto. apply Heqo1.
+               erewrite wf_asm_pc_repr; eauto.
+               generalize (Ptrofs.unsigned_range i0) (instr_size_positive i); omega.
+             }
+             {
+               exploit wf_asm_ret_jmp_comes_after_freeframe; eauto.
+               intros (o' & ifree & FI & IFREE & RNG).
+               generalize (find_instr_no_overlap _ _ _ _ _ FI Heqo0).
+               intro NOOV. trim NOOV. intro EQ; rewrite EQ in FI. rewrite FI in Heqo0; inv Heqo0. inv IFREE; inv CALL.
+               erewrite wf_asm_pc_repr in RNG; eauto. rewrite RNG in NOOV. 
+               generalize (instr_size_positive ifree) (instr_size_positive i); omega.
+             }
       + (* not a call, free ? *)
         destruct (is_free_dec i) as [(sz & ISFREE)|NISFREE].
         * inversion ISFREE; subst. clear NOTCALL.
@@ -440,8 +689,17 @@ Section SIMU.
           subst.
           destruct SPECi2 as [RET | JMP].
           -- subst. right.
-             eexists _, _; eapply step_free_ret. 4: apply STEP. 4: apply STEP2.
+             eexists _, _. split. eapply step_free_ret. 4: apply STEP. 4: apply STEP2.
              eauto. eauto. eauto.
+             exploit step_internal; eauto. intro IB; inv IB. intros (EI & T0).
+             simpl in EI. inv EI. unfold pc_at. destr. simpl in *. subst. simpl_regs.
+             exploit step_internal. apply STEP. eauto. intro IB; inv IB. intros (EI & _).
+             simpl in EI. repeat destr_in EI. simpl_regs. destr. inv Heqo.
+             destr. admit.
+             (* ret should jump right after a call instruction, i.e. not alloc
+             or ret or jmp. (jmp_s and jmp_r are used exclusively for tailcalls,
+             while jmp_l is used for "goto labels") -- not easy to ensure
+             because RA is stored in memory. --> ensure in the semantics ?*)
           -- exploit step_internal; eauto. intro IB; inv JMP; inv IB. intros (EI & T0).
              assert (PC3: exists i3,
                         pc_at ge s3 = Some i3 /\
@@ -477,35 +735,114 @@ Section SIMU.
              destruct SPECi3 as [(f' & ialloc & EQ & ALLOC)|(ef&EXT)]; subst.
              ++
                edestruct step_internal. apply STEP3. eauto. intro IB; inv IB; inv ALLOC. subst.
-               right; do 2 eexists. eapply step_free_tailcall.
+               right; do 2 eexists. split. eapply step_free_tailcall.
                apply PCs. apply PC2. apply PC3.
                all: eauto.
-             ++ right; do 2 eexists. eapply step_free_external.
+               unfold pc_at in PC3; repeat destr_in PC3.
+               unfold pc_at. destr. subst. simpl in H. inv ALLOC; simpl in H. repeat destr_in H.
+               simpl_regs. rewrite Heqv0. simpl. rewrite Heqo0. repeat destr.
+               intros. split; [intros f1 i1 EQ | intros ef EQ]; inv EQ.
+               intro A; inv A.
+               {
+                 inv H. exploit wf_asm_alloc_only_at_beginning. eauto. apply Heqo3.
+                 erewrite wf_asm_pc_repr; eauto. 
+                 generalize (Ptrofs.unsigned_range i) (instr_size_positive (Pallocframe f0 (Ptrofs.sub (Ptrofs.repr (align (frame_size (fn_frame f1)) 8)) (Ptrofs.repr (size_chunk Mptr)))) ); omega.
+               }
+               {
+                 exploit wf_asm_ret_jmp_comes_after_freeframe; eauto.
+                 intros (o' & ifree & FI & IFREE & RNG).
+                 generalize (find_instr_no_overlap' _ _ _ _ _ FI Heqo1). intros [EQ|NOOV].
+                 destruct H as [H|H]; subst; inv IFREE; inv H.
+                 erewrite wf_asm_pc_repr in RNG; eauto. rewrite <- RNG in NOOV.
+                 generalize (instr_size_positive (Pallocframe f0 (Ptrofs.sub (Ptrofs.repr (align (frame_size (fn_frame f1)) 8)) (Ptrofs.repr (size_chunk Mptr))))).
+                 generalize (instr_size_positive ifree). omega.
+               }
+
+             ++ right; do 2 eexists. split. eapply step_free_external.
                 apply PCs. apply PC2. apply PC3. all: eauto.
+                unfold pc_at in PC3; repeat destr_in PC3.
+                unfold pc_at. destr. subst.
+                inv STEP3; simpl in *; unfold ge in *; rewrite_hyps; try congruence.
+                simpl_regs.
+                assert (r RA = v).
+                edestruct step_internal. apply STEP2. eauto. intro IB; inv IB; inv JMP.
+                edestruct step_internal. apply STEP. eauto. intro IB; inv IB.
+                simpl in H3. rewrite Heqo in H3. inv H3.
+                inv JMP; simpl in H; repeat destr_in H. rewrite <- H6. simpl_regs. auto.
+                rewrite <- H6. simpl_regs. auto.
+                rewrite H.
+                (* ret should jump right after a call instruction, i.e. not alloc
+                   or ret or jmp. (jmp_s and jmp_r are used exclusively for tailcalls,
+                   while jmp_l is used for "goto labels") *)
+                admit.
+
         * (* not call nor free -> regular step *)
 
-          right; do 2 eexists.
+          right; do 2 eexists. split.
           eapply step_other. eauto.
           inversion 1; subst. intros f ISFREE; apply NISFREE. eauto.
+          intros. inv H. eapply INV. eauto. 
           inversion 1; subst; intros; eauto. eauto.
-    - right; do 2 eexists; eapply step_other; eauto.
-      inversion 1. inversion 1.
-    -
-      unfold pc_at in PCs. destr_in PCs. inv STEP; simpl in *; unfold ge in *.
-      + repeat destr_in PCs.
-      + repeat destr_in PCs.
-      + repeat destr_in PCs.
-  Qed.
+          destruct (is_builtin_dec i) as [IB|NIB].
+          -- unfold pc_at in PCs; repeat destr_in PCs.
+             simpl in STEP. inv STEP; unfold ge in *; rewrite_hyps; try congruence.
+             inv IB. simpl in H6. congruence.
+             simpl. simpl_regs.
+             rewrite set_res_other.
+             rewrite Asmgenproof0.undef_regs_other.
+             rewrite Heqv. simpl. rewrite Heqo.
+             destr. split;[intros f i0 EQ|intros eef EQ]; inv EQ.
+             intro II; inv II.
+             {
+               inv H. exploit wf_asm_alloc_only_at_beginning. eauto. apply Heqo1.
+               erewrite wf_asm_pc_repr; eauto.
+               generalize (Ptrofs.unsigned_range ofs) (instr_size_positive (Pbuiltin ef args res)); omega.
+             }
+             {
+               exploit wf_asm_ret_jmp_comes_after_freeframe; eauto.
+               intros (o' & ifree & FI & IFREE & RNG).
+               generalize (find_instr_no_overlap _ _ _ _ _ FI Heqo0).
+               intro NOOV. trim NOOV. intro EQ; rewrite EQ in FI. rewrite FI in Heqo0; inv Heqo0. inv IFREE; inv CALL.
+               erewrite wf_asm_pc_repr in RNG; eauto. rewrite RNG in NOOV. 
+               generalize (instr_size_positive ifree) (instr_size_positive (Pbuiltin ef args res)); omega.
+             }
+             {
+               intros r'  IN EQ; subst.
+               apply in_map_iff in IN. destruct IN as (mr & EQ & _).
+               eapply Asmgenproof0.preg_of_not_PC; eauto.
+             }
+             {
+               eapply wf_asm_builtin_not_PC; eauto.
+             }
+          -- edestruct step_internal. apply STEP. eauto. auto. subst.
+             specialize (INV _ _ eq_refl).
+             simpl in *.
+             fold ge in STEP.
+             eapply normal_steps_preserves_normal; eauto.
+
+    - edestruct INV2. eauto.
+    - unfold pc_at in PCs. destr_in PCs. inv STEP; simpl in *; unfold ge in *; repeat destr_in PCs.
+  Admitted.
 
   Theorem group_correct:
     forall rs,
       backward_simulation (RawAsm.semantics prog rs) (semantics prog rs).
   Proof.
     intro rs.
-    eapply backward_simulation_plus with (match_states := fun (s1 s2: Asm.state) => s1 = s2).
+    eapply backward_simulation_plus with (match_states := fun (s1 s2: Asm.state) =>
+                                                            s1 = s2 /\
+                                                            (forall f i, pc_at ge s1 = Some (inl (f, i)) -> ~ intermediate_instruction ge i)
+                                                            /\ ( forall ef, pc_at ge s1 = Some (inr ef) -> False)
+                                         ).
     - reflexivity.
     - intros; eauto.
-    - simpl; intros s1 s2 I1 I2. eauto.
+    - simpl; intros s1 s2 I1 I2. eexists; split. apply I1.
+      inv I1; inv I2. rewrite_hyps.
+      inv H0; inv H2. rewrite_hyps. split. unfold rs0, rs1. f_equal.
+      simpl. unfold rs0. simpl_regs.
+      unfold Genv.symbol_address.
+      eauto. split; eauto.
+      inv I2.
     - intros; subst. auto.
     - simpl; intros s1 s2 A SAFE; subst.
       edestruct SAFE; eauto. apply star_refl.
