x86/RawAsm.v
@@ -54,7 +54,7 @@ Section WITHGE.
     | Pret => Next (rs#PC <- (rs#RA) #RA <- Vundef) m
     | _ => Asm.exec_instr nil ge f i rs m
     end.
-  
+
   Inductive step  : state -> trace -> state -> Prop :=
   | exec_step_internal:
       forall b ofs f i rs m rs' m',
@@ -70,6 +70,7 @@ Section WITHGE.
         find_instr (Ptrofs.unsigned ofs) f.(fn_code) = Some (Pbuiltin ef args res) ->
         eval_builtin_args ge rs (rs RSP) m args vargs ->
         external_call ef ge vargs m t vres m' ->
+        ~ in_builtin_res res PC ->
         forall BUILTIN_ENABLED: builtin_enabled ef,
           rs' = nextinstr_nf
                   (set_res res vres
@@ -148,7 +149,7 @@ Section WITHMEMORYMODEL2.
       + discriminate.
       + discriminate.
       + assert (vargs0 = vargs) by (eapply Events.eval_builtin_args_determ; eauto). subst vargs0.
-        exploit Events.external_call_determ. eexact H5. eexact H11. intros [A B].
+        exploit Events.external_call_determ. eexact H5. eexact H12. intros [A B].
         split. auto. intros. destruct B; auto. subst. auto.
       + assert (args0 = args) by (eapply Asm.extcall_arguments_determ; eauto). subst args0.
         exploit Events.external_call_determ. eexact H4. eexact H9. intros [A B].
@@ -183,7 +184,7 @@ Section WITHMEMORYMODEL2.
       + discriminate.
       + discriminate.
       + assert (vargs0 = vargs) by (eapply Events.eval_builtin_args_determ; eauto). subst vargs0.
-        exploit Events.external_call_determ. eexact H5. eexact H11. intros [A B].
+        exploit Events.external_call_determ. eexact H5. eexact H12. intros [A B].
         split. auto. intros. destruct B; auto. subst. auto.
       + assert (args0 = args) by (eapply Asm.extcall_arguments_determ; eauto). subst args0.
         exploit Events.external_call_determ. eexact H4. eexact H9. intros [A B].
